Negative-Prove: the wrong equation in 2.7

src/common.lean
@@ -1,6 +1,42 @@
-import data.pnat.factors data.multiset
+import data.list data.list.sort data.bool
+import tactic.norm_num tactic.omega
+
+attribute [simp, reducible] nat.factors
+attribute [simp, reducible] ite
 
 notation `ℙ` := nat.primes
+
+set_option profiler true
+
+meta def by_eval (typ: Type*) [reflected typ]: tactic unit := do
+e <- tactic.target,
+match expr.is_eq e with
+| (some (e1, e2)) := tactic.eval_expr' typ e1 >> tactic.reflexivity
+| none := tactic.failed
+end
+
+namespace tree_sort
+
+inductive tree (α: Type*) --[has_lt α] [h : decidable_rel ((<) : α → α → Prop)]
+| l {} : tree
+| n : tree -> α -> tree -> tree
+
+@[simp, reducible]
+def tree.ins {α: Type*} (lt : α → α → bool) (x: α): tree α -> tree α
+| tree.l := tree.n tree.l x tree.l
+| (tree.n t y s) := cond (lt y x) (tree.n t y (tree.ins s)) (tree.n (tree.ins t) y s)
+
+@[simp, reducible]
+def tree.flat {α: Type*}: tree α -> list α
+| tree.l := []
+| (tree.n t x s) := (tree.flat t) ++ (x::(tree.flat s))
+
+@[simp, reducible]
+def sort {α: Type*}  (lt : α → α → bool) (l: list α) :=
+  tree.flat (list.foldl (λ t x, tree.ins lt x t) tree.l l)
+
+end tree_sort
+example: (tree_sort.sort (λ x y, to_bool (x < y)) (list.range 100)).length = 100 := by omega_nat ff
 
 -- 1-based
 def fib: nat -> nat
@@ -9,45 +45,72 @@ def fib: nat -> nat
 | 2 := 1
 | (n+2) := (fib (n)) + (fib (n+1))
 
+@[simp]
 def nat.sum (n: ℕ) := ((n+1)*n)/2
 
 -- seg a b = [a, ..., b)
+@[simp, reducible]
 def seg (a b: ℕ) := (list.range (b-a)).map(λ x, x+a)
 -- #eval seg 3 5 
 
+@[simp, reducible]
 def find {α: Type} (p: α -> Prop) [decidable_pred p] [inhabited α] : list α -> α
 | [] := arbitrary α
-| (h::t) := if p h then h else (find t)
+| (h::t) := cond (p h) h (find t)
 
--- prime_factors n = the set of prime factors of n
-def prime_factors (n: ℕ+) :=
-  (pnat.factor_multiset_equiv n).erase_dup
--- #eval prime_factors (2*2*3*5*5) -- = {2, 3, 5} (as primes, not ℕ+)
+@[simp, reducible]
+def list.uniq {α: Type*} [decidable_eq α]: list α -> list α
+| [] := []
+| [a] := [a]
+| (a::b::t) := cond (a = b) (list.uniq (b::t)) (a::(list.uniq (b::t)))
 
--- factorize n = the set of pairs {(p1, e1), ..., (pm, em)}, where Π pi^ei = n
-def factorize (n: ℕ+): multiset (ℙ × ℕ) := 
-  let m := pnat.factor_multiset_equiv n in 
-  let m' := m.map(fun x, (x, m.count x)) in
-  m'.erase_dup
--- #eval factorize (2*2*3*5*5) -- = {(2, 2), (3, 1), (5, 2)}
+-- factorize n = the list of pairs [(p1, e1), ..., (pm, em)], where Π pi^ei = n
+@[simp, reducible]
+def factorize (n: ℕ) : list (ℕ × ℕ) := 
+  let l := tree_sort.sort (λ a b, to_bool (a < b)) (nat.factors n) in
+  let (c: list ℕ) := list.map (λ x, list.count x l) l in
+  let l' := tree_sort.sort (λ a b, to_bool (a < b)) (list.zip l c) in
+  l'.uniq
 
--- ensure `factorize` is dupe-free
-theorem factorize_nodup: ∀ n, multiset.nodup (factorize n) := begin
-  intros; 
-  unfold factorize,
-  simp,
+#eval factorize (2*2*3*5*5)
+
+example: factorize (2*2*3*5*5) = [(2, 2), (3, 1), (5, 2)] := begin
+norm_num,
+reflexivity,
 end
 
-def divisors_factorized (n: ℕ+): multiset (multiset ℙ) := 
-  let m := pnat.factor_multiset_equiv n in
-  m.powerset.erase_dup
--- #eval divisors_ms (2*2*3*5*5) -- = {
-  -- {2, 2, 3, 5, 5}, {2, 2, 3, 5}, {2, 2, 3}, {2, 2, 5, 5}, 
-  -- {2, 2, 5}, {2, 2}, {2, 3, 5, 5}, {2, 3, 5}, 
-  -- {2, 3}, {2, 5, 5}, {2, 5}, {2}, {3, 5, 5}, {3, 5}, {3}, {5, 5}, {5}, {}
-  -- }
+@[simp, reducible]
+def list.subl {α: Type*} [has_lt α] [decidable_eq α] [decidable_rel ((<) : α → α → Prop)]: list α -> list (list α)
+| [] := [[]]
+| (h::t) := 
+  let sort := tree_sort.sort (λ (x y: list α), x.length < y.length) in
+  let ss := sort ((list.subl t) ++ (list.subl t).map(list.cons h)) in
+  (tree_sort.sort (λ (x y: list α), to_bool ((x.length, x) < (y.length, y))) ss).uniq
 
-def divisors (n: ℕ+) := 
-  let (m: multiset ℕ) := ↑(pnat.factor_multiset_equiv n) in
-  m.powerset.erase_dup.map(λ ns, multiset.fold (*) 1 ns)
--- #eval divisors (2*2*3*5*5) -- = {1, 2, 3, 4, 5, 6, 10, 12, 15, 20, 25, 30, 50, 60, 75, 100, 150, 300}
+#eval (nat.factors (2*2*3*5*5)).subl
+@[simp, reducible]
+def divisors_factorized (n: ℕ) :=
+  (tree_sort.sort (λ s t, (list.length s) < (list.length t)) (nat.factors n).subl)
+
+#eval divisors_factorized (2*2*3*5*5)
+example: divisors_factorized (2*2*3*5*5) = [
+  [], [5], [3], [2], [5, 5], [3, 5], [2, 5], [2, 3], 
+  [2, 2], [3, 5, 5], [2, 5, 5], [2, 3, 5], [2, 2, 5], [2, 2, 3], [2, 3, 5, 5], 
+  [2, 2, 5, 5], [2, 2, 3, 5], [2, 2, 3, 5, 5]
+] := begin
+norm_num,
+reflexivity,
+end 
+
+#eval divisors_factorized (2*2*3*5*5)
+
+@[simp, reducible]
+def divisors (n: ℕ) := 
+  tree_sort.sort (λ x y, to_bool (x < y)) ((divisors_factorized n).map list.prod)
+
+#eval divisors (2*2*3*5*5)
+example: divisors (2*2*3*5*5) = [1, 2, 3, 4, 5, 6, 10, 12, 15, 20, 25, 30, 50, 60, 75, 100, 150, 300] := begin
+norm_num,
+reflexivity,
+end
+
